Prove that `WPi` implies `wptp`.

src/handler.v
@@ -73,12 +73,12 @@ Qed.
 (** This class covers "sequential" [iHandler]s which are insensitive to the
 thread spawning continuation, that is, [iHandler]s that do not do concurrency. *)
 Class Sequential {Σ E} (H : iHandler Σ E) :=
-  is_seq : ∀ A e Φ s s', H A e Φ s -∗ H A e Φ s'.
+  is_seq : ∀ A e Φ s, H A e Φ s -∗ H A e Φ (const False).
 Global Instance sumH_Sequential {Σ E1 E2} (H1 : iHandler Σ E1) (H2 : iHandler Σ E2)
   `{!Sequential H1} `{!Sequential H2} :
   Sequential (H1 ⊕ H2).
 Proof.
-  iIntros (A e Φ s s') "HH". destruct e.
+  iIntros (A e Φ s) "HH". destruct e.
   - by iApply Sequential0.
   - by iApply Sequential1.
 Qed.
